added bb_type

theories/wz_bb.v
@@ -8,11 +8,26 @@ From Wasm Require Import datatypes list_extra.
 Import ListNotations.
 
 
-Inductive bb_type :=
+Inductive bb_t :=
   BB_unknown
   | BB_exit_end | BB_exit_return | BB_exit_unreachable
-  | BB_unreachable | BB_block | BB_loop | BB_if | BB_else | BB_end | BB_br | BB_br_if 
-  | BB_br_table | BB_return.
+  | BB_unreachable 
+  | BB_block | BB_loop 
+  | BB_if | BB_br | BB_br_if | BB_br_table | BB_return
+  | BB_code.
+
+Definition bb_t_of_instr (i: basic_instruction): bb_t :=
+  match i with
+  | BI_unreachable  => BB_unreachable
+  | BI_block _ _    => BB_unreachable
+  | BI_loop _ _     => BB_loop
+  | BI_if _ _ _     => BB_if
+  | BI_br _         => BB_br
+  | BI_br_if _      => BB_br_if
+  | BI_br_table _ _ => BB_br_table
+  | BI_return       => BB_return
+  | _               => BB_code
+  end.
 
 Inductive bb : Type :=
 {
@@ -21,7 +36,7 @@ Inductive bb : Type :=
 (*  mutable *) end_op:   nat;        (* index+1 of the last op in the expr *)
 (*  mutable *) succ:     list bb;    (* bblocks that can be directly reached from this bb *)
 (*  mutable *) pred:     list bb;    (* bblocks that can directly reach this bb *)
-(*  mutable *) bbtype:	 bb_type;    (* effectively the control opcode that created this bb *)
+(*  mutable *) bbtype:	 bb_t;       (* effectively the control opcode that created this bb *)
 (*  mutable *) nesting:  nat;        (* nesting level of the last opcode in the bb *)
 (*  mutable *) labels:   list nat;   (* destination labels used in BR, BR_IF, BR_TABLE instructions *)
 (*  mutable *) br_dest:	 option bb;  (* for LOOP, BLOCK and IF instructions the bb that's the target of a branch for this instruction  *)
@@ -30,6 +45,7 @@ Inductive bb : Type :=
 Inductive bb': Type :=
 {
   bb_index:   nat;
+  bb_type:    bb_t;
   bb_nesting: nat;
   bb_instrs:  list basic_instruction;
   bb_succ:    list bb';
@@ -42,9 +58,15 @@ Record bbs_progress: Type :=
     p_bbs:      list bb';
 }.
 
-Definition init_bb (idx: nat) (nesting: nat) (is: list basic_instruction): bb' :=
-  {| bb_index := idx; bb_nesting := nesting; bb_instrs := is; bb_succ := []; bb_pred := [] |}.
-Definition empty_bb (idx: nat) (nesting: nat): bb' := init_bb idx nesting [].
+Definition init_bb (idx: nat) (t: bb_t) (nesting: nat) (is: list basic_instruction): bb' :=
+  {|  bb_index    := idx;
+      bb_type     := t;
+      bb_nesting  := nesting;
+      bb_instrs   := is;
+      bb_succ     := []; 
+      bb_pred     := [] |}.
+
+Definition empty_bb (idx: nat) (nesting: nat): bb' := init_bb idx BB_code nesting [].
 
 Fixpoint bb's_of_expr' (bbs_prog: bbs_progress) (i: basic_instruction): bbs_progress :=
   let bb's_of_expr'' (bbs_prog: bbs_progress) (e: expr): bbs_progress :=
@@ -58,7 +80,7 @@ Fixpoint bb's_of_expr' (bbs_prog: bbs_progress) (i: basic_instruction): bbs_prog
       | [] => bbs_prog'
       (* yes, add it to the list of bbs *)
       | _ => {| p_bb  := empty_bb ((bb_index bb_acc)+1) (bb_nesting bb_acc);
-                p_bbs := ((init_bb (bb_index bb_acc) (bb_nesting bb_acc) (List.rev(bb_instrs bb_acc))))::bbs_acc |}
+                p_bbs := ((init_bb (bb_index bb_acc) BB_code (bb_nesting bb_acc) (List.rev(bb_instrs bb_acc))))::bbs_acc |}
       end
     in
     let bb_acc    := (p_bb  bbs_prog) in
@@ -70,6 +92,7 @@ Fixpoint bb's_of_expr' (bbs_prog: bbs_progress) (i: basic_instruction): bbs_prog
             {| p_bb   := empty_bb (bb_index (p_bb e1_p)) (bb_nesting bb_acc);
                p_bbs  := (p_bbs e1_p)
                           ++ (init_bb (bb_index bb_acc)
+                                      BB_block
                                       (bb_nesting bb_acc)
                                       (List.rev ((BI_block b [])::(bb_instrs bb_acc))))::bbs_acc |}
       | BI_loop b e1 =>
@@ -78,6 +101,7 @@ Fixpoint bb's_of_expr' (bbs_prog: bbs_progress) (i: basic_instruction): bbs_prog
             {| p_bb   := empty_bb (bb_index (p_bb e1_p)) (bb_nesting bb_acc);
                p_bbs  := (p_bbs e1_p)
                           ++ (init_bb (bb_index bb_acc)
+                                      BB_loop
                                       (bb_nesting bb_acc)
                                       (List.rev ((BI_loop b [])::(bb_instrs bb_acc))))::bbs_acc |}
       | BI_if b e1 e2 =>
@@ -88,6 +112,7 @@ Fixpoint bb's_of_expr' (bbs_prog: bbs_progress) (i: basic_instruction): bbs_prog
             {| p_bb   := (p_bb e2_p);
                p_bbs  := (p_bbs e2_p) ++ (p_bbs e2_p)
                           ++ (init_bb (bb_index (p_bb e2_p))
+                                      BB_if
                                       (bb_nesting (p_bb e2_p))
                                       (List.rev ((BI_loop b [])::(bb_instrs bb_acc))))::bbs_acc |}
     | BI_unreachable
@@ -97,25 +122,13 @@ Fixpoint bb's_of_expr' (bbs_prog: bbs_progress) (i: basic_instruction): bbs_prog
     | BI_return =>
         {|  p_bb  := empty_bb ((bb_index bb_acc)+1) (bb_nesting (p_bb bbs_prog));
             p_bbs := (init_bb (bb_index bb_acc)
+                              (bb_t_of_instr i)
                               (bb_nesting (p_bb bbs_prog))
                               (List.rev (i::(bb_instrs bb_acc))))::bbs_acc |}
     | _ => 
-        {|  p_bb  := init_bb ((bb_index bb_acc)) (bb_nesting (p_bb bbs_prog)) (i::(bb_instrs bb_acc));
+        {|  p_bb  := init_bb ((bb_index bb_acc)) BB_code (bb_nesting (p_bb bbs_prog)) (i::(bb_instrs bb_acc));
             p_bbs := bbs_acc |}
   end.
-
-Definition bb's_of_expr (e: expr): list bb' :=
-  let p := List.fold_left bb's_of_expr' e {| p_bb := empty_bb 0 0; p_bbs := [] |}
-  in
-    (* did we wind up having a bb at the end?*)
-    match bb_instrs (p_bb p) with
-    (* no, we're done *)
-    | [] => List.rev (p_bbs p)
-    (* yes, add it to the list of bbs*)
-    | _ => List.rev ((init_bb ((bb_index (p_bb p)))
-                              (bb_nesting (p_bb p))
-                              (List.rev (bb_instrs (p_bb p))))::(p_bbs p))
-    end.
 
 Definition succ_of_bbs (bbs: list bb'): list (list nat) :=
   let idx_of_else (idx: nat) (n: nat): option nat :=
@@ -152,20 +165,37 @@ Definition succ_of_bbs (bbs: list bb'): list (list nat) :=
   in
   mapi succ_of_bb bbs.
 
+Definition bb's_of_expr (e: expr): list bb' :=
+  let p := List.fold_left bb's_of_expr' e {| p_bb := empty_bb 0 0; p_bbs := [] |}
+  in
+    (* did we wind up having a bb at the end?*)
+    match bb_instrs (p_bb p) with
+    (* no, we're done *)
+    | [] => List.rev (p_bbs p)
+    (* yes, add it to the list of bbs*)
+    | _ => List.rev ((init_bb ((bb_index (p_bb p)))
+                              BB_code
+                              (bb_nesting (p_bb p))
+                              (List.rev (bb_instrs (p_bb p))))::(p_bbs p))
+    end.
+
+
 (* The simplest basic block *)
 Example simple_bb1 :
 forall (v1: value_num), 
   bb's_of_expr [BI_const_num v1] 
-  = [{| bb_index := 0; bb_nesting := 0; bb_instrs := [BI_const_num v1]; bb_pred := []; bb_succ := []|}].
+  = [{| bb_index := 0; bb_type := BB_code; bb_nesting := 0; bb_instrs := [BI_const_num v1]; bb_pred := []; bb_succ := []|}].
 Proof.
   compute. reflexivity.
 Qed.
+
+Definition i32_of n: i32 := Wasm_int.Int32.repr n.
 
 (* A slightly more complicated example*)
 Example simple_bb2 :
 forall (v1: value_num) (v2: value_num), 
   bb's_of_expr [BI_const_num v1; BI_const_num v2]
-  = [{| bb_index := 0; bb_nesting := 0; bb_instrs := [BI_const_num v1; BI_const_num v2]; bb_pred := []; bb_succ := [] |}].
+  = [{| bb_index := 0; bb_type := BB_code; bb_nesting := 0; bb_instrs := [BI_const_num v1; BI_const_num v2]; bb_pred := []; bb_succ := [] |}].
 Proof.
   reflexivity.
 Qed.
@@ -174,7 +204,7 @@ Qed.
 Example branch_bb1 :
 forall v1 v2 v3 l, 
   bb's_of_expr [BI_const_num v1; BI_const_num v2; BI_const_num v3; BI_br l]
-    = [{| bb_index := 0; bb_nesting := 0;
+    = [{| bb_index := 0; bb_type := BB_br; bb_nesting := 0;
           bb_instrs := [BI_const_num v1; BI_const_num v2; BI_const_num v3; BI_br l];
           bb_pred := []; bb_succ := [] |}].
 Proof.
@@ -184,17 +214,15 @@ Qed.
 Example branch_bb2 :
 forall v1 v2 v3 l, 
   bb's_of_expr [BI_const_num v1; BI_const_num v2; BI_br l; BI_const_num v3]
-  =   [ {|  bb_index := 0; bb_nesting := 0;
+  =   [ {|  bb_index := 0; bb_type := BB_br; bb_nesting := 0;
             bb_instrs := [BI_const_num v1; BI_const_num v2; BI_br l];
             bb_pred := []; bb_succ := [] |};
-        {|  bb_index := 1; bb_nesting := 0;
+        {|  bb_index := 1; bb_type := BB_code; bb_nesting := 0;
             bb_instrs := [BI_const_num v3];
             bb_pred := []; bb_succ := [] |}].
 Proof.
   compute. reflexivity.
 Qed.
-
-Definition i32_of n: i32 := Wasm_int.Int32.repr n.
 
 Definition bubble_sort_expr: expr :=
 [
@@ -279,13 +307,15 @@ Definition bubble_sort_expr: expr :=
     ]
 ].
 
+Compute succ_of_bbs (bb's_of_expr bubble_sort_expr).
+
 Definition bubble_sort_bbs: list bb' :=
-[ init_bb 0 0 [BI_block (BT_id 0%num) []];
-  init_bb 1 1 [BI_local_get 0%num;
+[ init_bb 0 BB_block 0 [BI_block (BT_id 0%num) []];
+  init_bb 1 BB_br_if 1 [BI_local_get 0%num;
           BI_const_num (VAL_int32 (i32_of 2));
           BI_relop T_i32 (Relop_i (ROI_lt SX_S));
           BI_br_if 0%num];
-  init_bb 2 1 [BI_local_get 0%num;
+  init_bb 2 BB_loop 1 [BI_local_get 0%num;
           BI_const_num (VAL_int32 (i32_of (-1)));
           BI_binop T_i32 (Binop_i BOI_add);
           BI_local_tee 2%num;
@@ -293,21 +323,21 @@ Definition bubble_sort_bbs: list bb' :=
           BI_const_num (VAL_int32 (i32_of 0));
           BI_local_set 4%num;
           BI_loop (BT_id 2%num) []];
-  init_bb 3 2 [BI_local_get 3%num;
+  init_bb 3 BB_block 2 [BI_local_get 3%num;
           BI_local_set 5%num;
           BI_const_num (VAL_int32 (i32_of 0));
           BI_local_set 6%num;
           BI_block (BT_id 0%num) []];
-  init_bb 4 3 [BI_local_get 4%num;
+  init_bb 4 BB_br_if 3 [BI_local_get 4%num;
           BI_local_tee 7%num;
           BI_local_get 0%num;
           BI_binop T_i32 (Binop_i BOI_sub);
           BI_const_num (VAL_int32 (i32_of (-2)));
           BI_relop T_i32 (Relop_i (ROI_gt SX_S));
           BI_br_if 0%num];
-  init_bb 5 3 [BI_loop (BT_id 4%num) []];
-  init_bb 6 4 [BI_block (BT_id 0%num) []];
-  init_bb 7 5 [BI_local_get 1%num;
+  init_bb 5 BB_loop 3 [BI_loop (BT_id 4%num) []];
+  init_bb 6 BB_block 4 [BI_block (BT_id 0%num) []];
+  init_bb 7 BB_br_if 5 [BI_local_get 1%num;
           BI_local_get 6%num;
           BI_local_tee 3%num;
           BI_const_num (VAL_int32 (i32_of 2));
@@ -329,19 +359,19 @@ Definition bubble_sort_bbs: list bb' :=
           BI_local_tee 9%num;
           BI_relop T_i32 (Relop_i (ROI_le SX_S));
           BI_br_if 0%num];
-  init_bb 8 5 [BI_local_get 6%num;
+  init_bb 8 BB_code 5 [BI_local_get 6%num;
           BI_local_get 9%num;
           BI_store T_i32 None {| memarg_offset := 0%num;  memarg_align := 0%num |};
           BI_local_get 8%num;
           BI_local_get 4%num;
           BI_store T_i32 None {| memarg_offset := 0%num;  memarg_align := 0%num |}];
-  init_bb 9 4 [BI_local_get 3%num;
+  init_bb 9 BB_br_if 4 [BI_local_get 3%num;
           BI_local_set 6%num;
           BI_local_get 3%num;
           BI_local_get 5%num;
           BI_relop T_i32 (Relop_i ROI_ne);
           BI_br_if 0%num];
-  init_bb 10 1 [BI_local_get 5%num;
+  init_bb 10 BB_br_if 1 [BI_local_get 5%num;
           BI_const_num (VAL_int32 (i32_of (-1)));
           BI_binop T_i32 (Binop_i BOI_add);
           BI_local_set 3%num;
